[OK] skeleton for lt2

theories/l2t.v
@@ -1,10 +1,10 @@
 From mathcomp Require Import all_ssreflect.
-From det Require Import lang run run_prop valid_state elpi elpi_equiv elpi_prop.
+From det Require Import lang run run_prop valid_state elpi elpi_equiv elpi_prop run_prop_hard.
 From elpi.apps Require Import derive derive.std.
 From HB Require Import structures.
 From det Require Import zify_ssreflect.
 
-Fixpoint l2t_alts (a : alts) : state :=
+(* Fixpoint l2t_alts (a : alts) : state :=
   match a with
   | no_alt => Bot
   | more_alt (s,gl) a => Or Bot s (Or (l2t_goals gl) s (l2t_alts a))
@@ -18,25 +18,172 @@ with l2t_G g :=
   match g with
   | call p c => CallS p c
   | cut _ => CutS
-  end.
+  end. *)
 
+Lemma s2l_nil_is_ko u {A s1 bt}:
+  valid_state A ->
+  state_to_list A s1 bt = nilC ->
+    forall s, dead_run u s A.
+Proof.
+  elim: A s1 bt => //=.
+  - move=> ???????? H.
+    apply: is_ko_runb _ _ H => //.
+  - move=> A HA s B HB s1 bt; case: ifP => [dA vB|dA /andP[vA bB]].
+      rewrite state_to_list_dead => //.
+      case X: state_to_list => [|[]]// _ s2 s3 r b H.
+      have [[A' [b' H1]]|[B'[b' H1]]]:= run_or_complete _ H.
+        by apply: is_dead_runb dA H1.
+      by apply: HB H1; eauto.
+    case X: state_to_list => [|[]]//.
+    case Y: state_to_list => [|[]]// _.
+    move=> s2 s3 r b H.
+    have [[A' [b' H1]]|[B'[b' H1]]]:= run_or_complete _ H.
+      by apply: HA H1; eauto.
+    by apply: HB H1; eauto; apply: bbOr_valid bB.
+  - move=> A HA B0 HB0 B HB s1 bt /and5P[_ vA _].
+    case: ifP => /=[sA vB bB0|sA/eqP->{HB0}].
+      rewrite (success_state_to_list s1)//=. (*TODO: not sure it is s1*)
+      move/orP: bB0 => []bB; last first.
+        rewrite base_and_ko_state_to_list//=.
+        case X: state_to_list => //= _ s2 s3 r b H1.
+        have {}HB := HB _ _ vB X.
+        have {}HB0 := HB0 empty no_alt (base_and_ko_valid bB) (base_and_ko_state_to_list bB).
+        admit. (*should be ok: but B and B0 fail*)
+      have [hd H]:= base_and_state_to_list bB; rewrite H/=.
+      case X: state_to_list => //.
+      case Y: state_to_list => [|[]]// _ s2 s3 r b H1.
+      have {}HB := HB _ _ vB X.
+      admit. (*should be ok: A success, B fails and A has no alternatives*)
+    case: ifP => [fA bB|fA bB].
+      case X: state_to_list => [|[s2 x]xs].
+        move=> _ s3 s4 r b H.
+        have [sm[r1[b1 H1]]]:= run_and_correct _ H.
+        by apply: HA H1; eauto.
+      move/orP: bB => []bB; last first.
+        rewrite base_and_ko_state_to_list//=.
+        case Y: state_to_list => //= _ s4 s5 r b H1.
+        have {}HB := HB _ _ (base_and_ko_valid bB) Y.
+        admit. (*should be ok: A is any, B and B0 (which is equal to B) fail*)
+      have [hd H]:= base_and_state_to_list bB; rewrite H/=H//=.
+    case X: state_to_list => [|[s2 x]xs].
+      move=> _ s3 s4 r b H.
+      have [sm[r1[b1 H1]]]:= run_and_correct _ H.
+      by apply: HA H1; eauto.
+    have [hd H]:= base_and_state_to_list bB; rewrite H/=H//=.
+Admitted.
+
+
+Lemma state_to_list_success {u A s s1 bt xs}:
+  state_to_list A s bt = (s1, nilC) ::: xs ->
+    Texists A', expandedb u s A (Done (get_substS s A) A') 0. (*TODO: specify better A'*)
+Proof.
+  elim: A s s1 bt xs => //=.
+  - move=> s s1 _ []// _; eexists; apply: expanded_done => //.
+  - move=> s s1 _ []// _; eexists; apply: expanded_step => //; apply: expanded_done => //.
+  - move=> A HA s B HB s1 s2 bt xs.
+    rewrite add_ca_deep_cat.
+    case X: state_to_list => [|[s3 y]ys].
+      rewrite cat0s.
+      case Y: state_to_list => [|[s4 [|??]]zs]//[??]; subst.
+      move: Y; fNilG; fConsA (s1, nilC) zs => Y.
+      have {HA HB} [b1 H] := HB _ _ _ _ Y.
+Abort.
+
+Lemma s2l_add_ca {A s bt1 xs}:
+  state_to_list A s bt1 = add_ca_deep bt1 xs ->
+    forall bt2, state_to_list A s bt2 = add_ca_deep bt2 xs.
+Proof.
+  elim: A s bt1 xs => //=.
+  - by move=> _ bt1 []//=[]//.
+  - by move=> s bt1 []//=[]//a[]//[]//[]//.
+  - by move=> s bt []//[]/=a []//=[]//[]//.
+  - by move=> _ bt1 []//[]//.
+  - by move=> p c s bt []//[]// a []//= []//= p1 c1 []//[]//[]//.
+  - move=> s bt []//[]// s1 []// []//= [|[]]//=[]//[|[]]//; case: bt => //=.
+Abort.
+
+Definition add_ca_deep_lvl1 (bt:alts) (a: alts) : alts := 
+  map (fun '(s,xs) => (s,map (apply_cut (fun ca => add_ca_deep bt ca)) xs)) a.
+
+Lemma split_cat {x1 x2: alts} {F r}:
+  x1 ++ x2 = map F r -> Texists p1 p2, p1 ++ p2 = r /\ x1 = map F p1 /\ x2 = map F p2.
+Proof.
+Admitted.
+
+(* Lemma s2l_add_ca {A s xs bt1}:
+  state_to_list A s bt1 = add_ca_deep_lvl1 bt1 xs ->
+    forall bt2, state_to_list A s bt2 = add_ca_deep_lvl1 bt2 xs.
+Proof.
+  (* rewrite /add_ca_deep_lvl1. *)
+  elim: A s xs bt1 => //=.
+  - by move=> _ [|[]]//=.
+  - by move=> s [|[]]//= s1 []//[|[]]//.
+  - by move=> s []//[]s1 []//=[]//.
+  - by move=> _ []//.
+  - by move=> p c s []//= []s1 []//=[]//p1 c1[]//[]//.
+  - by move=> s []//[]//=s1 []//= []//= [|[]]// []//[]//.
+  - move=> A HA s1 B HB s2 xs bt1 + bt2.
+    rewrite !add_ca_deep_cat.
+    have:= HA s2 _ (state_to_list B s1 nilC) => /(_ _ _ IsList_alts).
+    set X:= state_to_list A _ _.
+    have:= HB s1 _ nilC => /(_ _ _ IsList_alts).
+    set Z:= state_to_list B _ _.
+    move=> {}HB {}HA.
+    admit.
+  - move=> A HA B0 HB0 B HB s1 xs bt1 + bt2.
+
+
+Abort. *)
+
+Lemma xx {u A s s1 bt xs}:
+  valid_state A ->
+  state_to_list A s bt = (s1, nilC) ::: xs ->
+  Texists B n,
+    runb u s A s1 B n 
+    (* /\  *)
+    (* state_to_list (odflt Bot B) s bt2 = add_ca_deep bt2 a *)
+    .
+Proof.
+  elim: A s s1 bt xs => //=.
+  - move=> s s1 bt [|[]]//= _ [->].
+    repeat eexists.
+      apply: run_done (expanded_done _ _) _ => //.
+    (* move=> //. *)
+  - move=> s s1 bt [|[]]//= _ [->]; repeat eexists.
+      apply: run_done (expanded_step _ _ (expanded_done _ _)) _ => //.
+    (* move=>//. *)
+  - move=> A HA s B HB s1 s2 bt a.
+    rewrite add_ca_deep_cat.
+    case:ifP => [dA vB|dA /andP[vA bB]].
+      rewrite state_to_list_dead//=.
+      case X: state_to_list => //[[s3 [|??]]xs]//=[? H]; subst.
+      move: X; fNilG; fConsA (s2, nilC) xs => X.
+      have {HB} := [elaborate HB s s2 nilC xs vB X].
+      move=> [r [n H]].
+      have [r''[H3 H4]] := run_ko_left2 _ s1 (is_dead_is_ko dA) H.
+      repeat eexists; eauto.
+    case X: state_to_list => [|[sx x]xs].
+      fNilA; case Y: state_to_list => //[[s3 [|??]]ys]//[??]; subst.
+      move: Y; fNilG; fConsA (s2, nilC) ys => Y.
+      have H := s2l_nil_is_ko u vA X s1.
+      (* have:=  *)
+Admitted.
+    
 
 Lemma two' {u s s1} {alts alts_left : alts} {andg : goals}  : 
-  nur u s andg alts s1 alts_left -> forall t bt bt1,
+  nur u s andg alts s1 alts_left -> forall t bt,
+  valid_state t ->
   state_to_list t s bt = add_ca_deep bt ((s,andg) ::: alts) -> 
   Texists t1 n,
-  state_to_list (odflt Bot t1) s1 bt1 = add_ca_deep bt1 alts_left /\ runb u s t s1 t1 n.
+    runb u s t s1 t1 n
+      (* /\ state_to_list (odflt Bot t1) s1 bt1 = add_ca_deep bt1 alts_left  *)
+    .
 Proof.
   elim; clear.
 
-  - move=> s a t bt1 bt2 Ht.
-    exists (Some (l2t_alts a)), 0 => /=.
-    split; last first.
-      apply: run_done.
-      admit.
-      admit.
-    admit.
-  - move=> s1 s2 a ca r gl H IH t H1.
+  - move=> s a t bt1 /= vt Ht.
+    apply: xx vt Ht.
+  - move=> s1 s2 a ca r gl H IH t bt H1.
     admit.
   - admit.
   - admit.
@@ -45,11 +192,13 @@ Admitted.
 
 Lemma two'' {u s s1} {alts alts_left : alts} {andg : goals}  : 
   nur u s andg alts s1 alts_left -> forall t,
+  valid_state t ->
   state_to_list t s nilC = ((s,andg) ::: alts) -> 
   Texists t1 n,
-  state_to_list (odflt Bot t1) s1 nilC = alts_left /\ runb u s t s1 t1 n.
-move=> H t H1.
-have:= [elaborate (two' H t nilC nilC)].
+  (* state_to_list (odflt Bot t1) s1 nilC = alts_left /\  *)
+  runb u s t s1 t1 n.
+move=> H t vt H1.
+have:= [elaborate (two' H t nilC vt)].
 by rewrite !add_ca_deep_empty1; auto.
 Qed.
 
